links: add dependencies for chainid

CoqOfRust/revm/revm_context_interface/links/cfg.v
@@ -1,6 +1,8 @@
 Require Import CoqOfRust.CoqOfRust.
 Require Import CoqOfRust.links.M.
+Require Import CoqOfRust.core.convert.links.mod.
 Require Import CoqOfRust.revm.links.dependencies.
+Require Import CoqOfRust.revm.revm_specification.links.hardfork.
 
 (*
   /// Create scheme.
@@ -38,25 +40,13 @@ pub trait Cfg {
     type Spec: Into<SpecId> + Clone;
 
     fn chain_id(&self) -> u64;
-
-    // Specification id that is set.
     fn spec(&self) -> Self::Spec;
-
-    /// Returns the blob target and max count for the given spec id.
-    ///
-    /// EIP-7840: Add blob schedule to execution client configuration files
     fn blob_max_count(&self, spec_id: SpecId) -> u8;
-
     fn max_code_size(&self) -> usize;
-
     fn is_eip3607_disabled(&self) -> bool;
-
     fn is_balance_check_disabled(&self) -> bool;
-
     fn is_block_gas_limit_disabled(&self) -> bool;
-
     fn is_nonce_check_disabled(&self) -> bool;
-
     fn is_base_fee_check_disabled(&self) -> bool;
 }
 *)
@@ -67,7 +57,6 @@ Module Cfg.
       Spec : Set;
     }.
 
-    
     Class AreLinks (types : t) : Set := {
       H_Spec : Link types.(Spec);
     }.
@@ -83,15 +72,132 @@ Module Cfg.
         {{ chain_id [] [] [ φ self ] 🔽 U64.t }}
     }.
 
-  (* NOTE: Is this the right design for `Run`'s parameters? *)
-  Record Run (Self : Set) `{Link Self} (types : Types.t) 
-    `{Types.AreLinks types} : Set := 
+  Definition Run_spec (Self : Set) `{Link Self} (types : Types.t) `{Types.AreLinks types} : Set :=
+    {spec @
+      IsTraitMethod.t "revm_context_interface::cfg::Cfg" [] [] (Φ Self) "spec" spec *
+      forall (self : Ref.t Pointer.Kind.Ref Self),
+        {{ spec [] [] [ φ self ] 🔽 types.(Types.Spec) }}
+    }.
+
+  Definition Run_blob_max_count (Self : Set) `{Link Self} (types : Types.t) `{Types.AreLinks types} : Set :=
+    {blob_max_count @
+      IsTraitMethod.t "revm_context_interface::cfg::Cfg" [] [] (Φ Self) "blob_max_count" blob_max_count *
+      forall (self : Ref.t Pointer.Kind.Ref Self) (spec_id : SpecId.t),
+        {{ blob_max_count [] [] [ φ self; φ spec_id ] 🔽 U8.t }}
+    }.
+
+  Definition Run_max_code_size (Self : Set) `{Link Self} : Set :=
+    {max_code_size @
+      IsTraitMethod.t "revm_context_interface::cfg::Cfg" [] [] (Φ Self) "max_code_size" max_code_size *
+      forall (self : Ref.t Pointer.Kind.Ref Self),
+        {{ max_code_size [] [] [ φ self ] 🔽 Usize.t }}
+    }.
+
+  Definition Run_is_eip3607_disabled (Self : Set) `{Link Self} : Set :=
+    {is_eip3607_disabled @
+      IsTraitMethod.t "revm_context_interface::cfg::Cfg" [] [] (Φ Self) "is_eip3607_disabled" is_eip3607_disabled *
+      forall (self : Ref.t Pointer.Kind.Ref Self),
+        {{ is_eip3607_disabled [] [] [ φ self ] 🔽 bool }}
+    }.
+
+  Definition Run_is_balance_check_disabled (Self : Set) `{Link Self} : Set :=
+    {is_balance_check_disabled @
+      IsTraitMethod.t "revm_context_interface::cfg::Cfg" [] [] (Φ Self) "is_balance_check_disabled" is_balance_check_disabled *
+      forall (self : Ref.t Pointer.Kind.Ref Self),
+        {{ is_balance_check_disabled [] [] [ φ self ] 🔽 bool }}
+    }.
+
+  Definition Run_is_block_gas_limit_disabled (Self : Set) `{Link Self} : Set :=
+    {is_block_gas_limit_disabled @
+      IsTraitMethod.t "revm_context_interface::cfg::Cfg" [] [] (Φ Self) "is_block_gas_limit_disabled" is_block_gas_limit_disabled *
+      forall (self : Ref.t Pointer.Kind.Ref Self),
+        {{ is_block_gas_limit_disabled [] [] [ φ self ] 🔽 bool }}
+    }.
+
+  Definition Run_is_nonce_check_disabled (Self : Set) `{Link Self} : Set :=
+    {is_nonce_check_disabled @
+      IsTraitMethod.t "revm_context_interface::cfg::Cfg" [] [] (Φ Self) "is_nonce_check_disabled" is_nonce_check_disabled *
+      forall (self : Ref.t Pointer.Kind.Ref Self),
+        {{ is_nonce_check_disabled [] [] [ φ self ] 🔽 bool }}
+    }.
+
+  Definition Run_is_base_fee_check_disabled (Self : Set) `{Link Self} : Set :=
+    {is_base_fee_check_disabled @
+      IsTraitMethod.t "revm_context_interface::cfg::Cfg" [] [] (Φ Self) "is_base_fee_check_disabled" is_base_fee_check_disabled *
+      forall (self : Ref.t Pointer.Kind.Ref Self),
+        {{ is_base_fee_check_disabled [] [] [ φ self ] 🔽 bool }}
+    }.
+
+  Record Run (Self : Set) `{Link Self} (types : Types.t)  `{Types.AreLinks types} : Set :=
   {
     Spec_IsAssociated :
       IsTraitAssociatedType
         "revm_context_interface::cfg::Cfg" [] [] (Φ Self)
         "Spec" (Φ types.(Types.Spec));
-    (* run_StackTrait_for_Stack : StackTrait.Run types.(Types.Stack); *) (* TODO: Do we need to implement `Into` for Spec? *)
+    run_Into_for_Spec : Into.Run types.(Types.Spec) SpecId.t;
     chain_id : Run_chain_id Self;
+    spec : Run_spec Self types;
+    blob_max_count : Run_blob_max_count Self types;
+    max_code_size : Run_max_code_size Self;
+    is_eip3607_disabled : Run_is_eip3607_disabled Self;
+    is_balance_check_disabled : Run_is_balance_check_disabled Self;
+    is_block_gas_limit_disabled : Run_is_block_gas_limit_disabled Self;
+    is_nonce_check_disabled : Run_is_nonce_check_disabled Self;
+    is_base_fee_check_disabled : Run_is_base_fee_check_disabled Self;
   }.
 End Cfg.
+
+(*
+pub trait CfgGetter {
+    type Cfg: Cfg;
+
+    fn cfg(&self) -> &Self::Cfg;
+}
+*)
+Module CfgGetter.
+  Module Types.
+    Record t : Type := {
+      Cfg : Set;
+      Spec : Set;
+    }.
+
+    Class AreLinks (types : t) : Set := {
+      H_Cfg : Link types.(Cfg);
+      H_Spec : Link types.(Spec);
+    }.
+
+    Global Instance IsLinkCfg (types : t) (H : AreLinks types) : Link types.(Cfg) :=
+      H.(H_Cfg _).
+
+    Global Instance IsLinkSpec (types : t) (H : AreLinks types) : Link types.(Spec) :=
+      H.(H_Spec _).
+
+    Definition to_Cfg_types (types : t) : Cfg.Types.t :=
+      {|
+        Cfg.Types.Spec := types.(Spec);
+      |}.
+
+    Global Instance AreLinks_to_Cfg_types (types : t) (H : AreLinks types) :
+      Cfg.Types.AreLinks (to_Cfg_types types) :=
+      {|
+        Cfg.Types.H_Spec := _;
+      |}.
+  End Types.
+
+  Definition Run_cfg (Self : Set) `{Link Self} (types : Types.t) `{Types.AreLinks types} : Set :=
+    {cfg @
+      IsTraitMethod.t "revm_context_interface::cfg::CfgGetter" [] [] (Φ Self) "cfg" cfg *
+      forall (self : Ref.t Pointer.Kind.Ref Self),
+        {{ cfg [] [] [ φ self ] 🔽 Ref.t Pointer.Kind.Ref types.(Types.Cfg) }}
+    }.
+
+  Record Run (Self : Set) `{Link Self} (types : Types.t) `{Types.AreLinks types} : Set :=
+  {
+    Cfg_IsAssociated :
+      IsTraitAssociatedType
+        "revm_context_interface::cfg::CfgGetter" [] [] (Φ Self)
+        "Cfg" (Φ types.(Types.Cfg));
+    run_Cfg_for_Cfg : Cfg.Run types.(Types.Cfg) (Types.to_Cfg_types types);
+    cfg : Run_cfg Self types;
+  }.
+End CfgGetter.
